verification/proofs/Chunk_hexVal/obl_0_17_0.lean
@@ -1,4 +1,4 @@
-  simp only [inv_22, inv_41, inv_60, inv_64]
+  simp only [inv_17, inv_36, inv_55, inv_59]
   simp [run, step, P, hpc, hstk, State.set, pLt, pGt, *] at hrun
   subst hrun
   simp only [State.set, Nat.reduceEqDiff, reduceIte]
